\begin{frame}[fragile]
\frametitle{Another solution with Dependent Types}

\begin{lstlisting}[frame=single]
v : Vect n a -> (v ++ Nil) = v
\end{lstlisting}

\begin{lstlisting}[frame=single]
v : Vect n a -> (Nil ++ v) = v
\end{lstlisting}

\begin{lstlisting}[frame=single]
v : Vect n a ->
w : Vect n a ->
x : Vect n a ->
(v ++ w) ++ x = v ++ w ++ x
\end{lstlisting}

\begin{lstlisting}[frame=single]
v : Vect n a ->
w : Vect n a ->
x : Vect n a ->
v ++ (w ++ x) = v ++ w ++ x
\end{lstlisting}

\begin{lstlisting}[frame=single]
Proofs of these propositions.
\end{lstlisting}

\end{frame}
